src/Std/Data/Iterators.lean
@@ -8,6 +8,7 @@ import Std.Data.Iterators.Basic
 import Std.Data.Iterators.Producers
 import Std.Data.Iterators.Consumers
 import Std.Data.Iterators.Internal
+import Std.Data.Iterators.Lemmas
 
 /-!
 # Iterators
